Partial progress on interface to source_evalProof
The plan is to make source_evalProof present an interface that
asks for the kinds of things the translator will actually provide,
rather than various layers of construction of the necessary
parameters. This creates various headaches. Progress in continuing.

compiler/backend/proofs/backendProofScript.sml
@@ -27,7 +27,8 @@ val _ = set_trace "BasicProvers.var_eq_old" 1
 val _ = Parse.set_grammar_ancestry
   [ "backend", "backend_common", "backendProps",
     "primSemEnv", "semanticsProps",
-    "labProps" (* for good_dimindex *)
+    "labProps", (* for good_dimindex *)
+    "source_evalProof" (* for compiler instance structure *)
   ];
 
 (* TODO: move/rephrase *)
@@ -2522,18 +2523,13 @@ Proof
   \\ drule_then (simp o single) cake_orac_config_eqs
 QED
 
-val _ = Datatype `backend_eval_config =
-  <| decode_v : semanticPrimitives$v -> ('a config) option
-   ; encode_v : 'a config -> semanticPrimitives$v
-  |>`;
-
 Definition match_decode_config_def:
-  match_decode_config ec c v = (ec.decode_v v = SOME c)
+  match_decode_config ci c v = ci.config_v_rel c v
 End
 
 Definition eval_config_compile_def:
   eval_config_compile ec x = let (env_id, c_v, decs) = x in
-  case ec.decode_v c_v of
+  case v_rel_abs ec.config_v_rel c_v of
     NONE => NONE
   | SOME c' => let (c'', ps) = compile_inc_progs c' (env_id, decs) in
     OPTION_MAP (\(bs, ws). (match_decode_config ec c'', bs,
@@ -2543,7 +2539,7 @@ End
 
 Theorem eval_config_compile_backend_compile_inc_progs:
   eval_config_compile ec x = let (env_id, c_v, decs) = x in
-  case ec.decode_v c_v of
+  case v_rel_abs ec.config_v_rel c_v of
     NONE => NONE
   | SOME c' => let (c'', ps) = backend_compile_inc_progs c' (env_id, decs) in
     OPTION_MAP (\(bs, ws). (match_decode_config ec c'', bs,
@@ -2557,15 +2553,15 @@ QED
 
 Definition eval_config_cfg_compile_def:
   eval_config_cfg_compile ec x = let (env_id, c_v, decs) = x in
-  case ec.decode_v c_v of
+  case v_rel_abs ec.config_v_rel c_v of
   | SOME c' => let (c'', ps) = compile_inc_progs c' (env_id, decs) in
-    ec.encode_v c''
+    v_rel_conc ec.config_v_rel c''
 End
 
 Theorem eval_config_compilers_equiv:
   eval_config_compile ec args = SOME res ==>
   ?cfg prog. res = (match_decode_config ec cfg, prog) /\
-  eval_config_cfg_compile ec args = ec.encode_v cfg
+  eval_config_cfg_compile ec args = v_rel_conc ec.config_v_rel cfg
 Proof
   PairCases_on `args`
   \\ simp [eval_config_compile_def, option_case_eq, eval_config_cfg_compile_def]
@@ -2573,30 +2569,12 @@ Proof
   \\ metis_tac []
 QED
 
-Definition eval_config_to_eval_state_def:
-  eval_config_to_eval_state c ec = EvalDecs
-  <| compiler := eval_config_compile ec
-   ; compiler_state := match_decode_config ec c
-   ; env_id_counter := (0, 0, 1)
-  |>
-End
-
-Definition K_same_type_def:
-  (K_same_type : 'a -> 'a -> 'a) x y = x
-End
-
-Definition eval_config_to_interp_def:
-  eval_config_to_interp ec =
-    source_to_flatProof$update_decode_state
-      (λv. case ec.decode_v v of
-           | NONE => NONE
-           | SOME c => SOME (config_tuple1 c)) ARB
-End
-
 Definition add_eval_state_def:
   add_eval_state NONE c s0 = s0 /\
-  add_eval_state (SOME ev) c s0 =
-    s0 with <| eval_state := SOME (eval_config_to_eval_state c ev) |>
+  add_eval_state (SOME ci) c s0 =
+    s0 with <| eval_state := SOME (mk_init_eval_state
+        (ci with <| init_state := (c, THE (v_rel_conc ci.config_v_rel c)) |> ))
+    |>
 End
 
 Theorem add_eval_state_ffi:
@@ -2605,8 +2583,18 @@ Proof
   Cases_on `opt_ev` \\ simp [add_eval_state_def]
 QED
 
+Definition compile_inc_progs_st_fun_def:
+  compile_inc_progs_st_fun x =
+  let (env_id, c', decs) = x in
+  let (c'', ps) = compile_inc_progs c' (env_id, decs) in
+    OPTION_MAP (\(bs, ws). (c'', bs,
+            MAP data_to_word_gcProof$upper_w2w (DROP (LENGTH c'.word_conf.bitmaps) ws)))
+        ps.target_prog
+End
+
 Definition opt_eval_config_wf_def:
-  opt_eval_config_wf (SOME ec) = (!cfg. ec.decode_v (ec.encode_v cfg) = SOME cfg) /\
+  opt_eval_config_wf (SOME ci) = (ci.compiler_fun = compile_inc_progs_st_fun /\
+    (!v cfg cfg2.  ci.config_v_rel v cfg /\ ci.config_v_rel v cfg2 ==> cfg2 = cfg)) /\
   opt_eval_config_wf NONE = T
 End
 
@@ -2729,6 +2717,7 @@ Proof
   simp [FUN_EQ_THM, cake_orac_def, UNCURRY]
 QED
 
+(*
 Theorem mk_orac_st_eq_cake_orac:
   ~ semantics_prog (s1 with eval_state := SOME (eval_config_to_eval_state c ev)) env decs Fail /\
   s1.refs = [] /\
@@ -2785,10 +2774,44 @@ Proof
   \\ rveq \\ fs []
   \\ simp [compile_inc_progs_src_env]
 QED
+*)
 
 Overload "mk_flat_install_conf" = “flatProps$mk_flat_install_conf”;
 
 val mk_flat_install_conf_def = flatPropsTheory.mk_flat_install_conf_def;
+
+Theorem config_wf_abs_conc:
+
+  opt_eval_config_wf (SOME ci) ==>
+  v_rel_abs ci.config_v_rel (THE (v_rel_conc ci.config_v_rel cfg)) = SOME cfg
+
+Proof
+
+  simp [opt_eval_config_wf_def, source_evalProofTheory.v_rel_abs, 
+    source_evalProofTheory.v_rel_conc]
+
+Triviality cake_orac_extended_wf:
+
+  opt_eval_config_wf (SOME ci) ==>
+  orac_extended_wf (mk_compiler_fun_from_ci ci)
+    ((λ(cfg,id,ds). (id,THE (v_rel_conc x.config_v_rel cfg),ds)) ∘
+    cake_orac c' syntax I (λps. (ps.env_id,ps.source_prog)))
+
+Proof
+
+  rw [source_evalProofTheory.orac_extended_wf_def, cake_orac_SUC]
+  \\ rpt (pairarg_tac \\ fs [])
+  \\ fs [source_evalProofTheory.mk_compiler_fun_from_ci_def]
+  \\ rpt (pairarg_tac \\ fs [])
+  \\ rveq \\ fs []
+  \\ fs [cake_orac_def, UNCURRY, compile_inc_progs_src_env]
+  \\ rveq \\ fs []
+  \\ rfs [opt_eval_config_wf_def, compile_inc_progs_st_fun_def]
+  \\ rpt (pairarg_tac \\ fs [])
+  \\ rveq \\ fs []
+
+  simp [
+
 
 Theorem source_eval_semantics:
   ~ semantics_prog (add_eval_state ev c' s0) env prog Fail /\
@@ -2803,10 +2826,19 @@ Theorem source_eval_semantics:
         (backend_from_flat_tuple_cc c)
         (cake_orac c' syntax_oracle (SND o config_tuple1) (\ps. ps.flat_prog)))
     s0.ffi p')
+
 Proof
+
   rw []
-  \\ qabbrev_tac `es = source_evalProof$mk_orac_st (eval_config_cfg_compile (THE ev))
-        ((THE ev).encode_v c') (add_eval_state ev c' s0) env prog`
+  \\ qabbrev_tac `adj = (\po.
+        (\(cfg, id, ds). (id, THE (v_rel_conc (THE ev).config_v_rel cfg), ds))
+            o
+        cake_orac c'
+            (\i. case po i of SOME (id, (v : v), ds) => (id, ds)
+                | _ => ((0, 0), []))
+            I (\ps. (ps.env_id,ps.source_prog)))`
+  \\ qabbrev_tac `es = source_evalProof$mk_orac_st adj
+        (THE ev) (add_eval_state ev c' s0) env prog`
   \\ qexists_tac `(I ## SND) o ((source_evalProof$orac_s es).oracle)`
   \\ fs [Q.ISPEC `compile prim_src_config _` PAIR_FST_SND_EQ]
   \\ rveq \\ fs []
@@ -2843,16 +2875,67 @@ Proof
     \\ EVAL_TAC
   )
   \\ fs [add_eval_state_def]
-  \\ drule_then irule source_evalProofTheory.oracle_semantics_prog
+
+  \\ qspec_then `the_ev` (drule_then irule)
+    (source_evalProofTheory.oracle_semantics_prog
+        |> INST_TYPE [``:'a`` |-> ``:'z``] |> Q.GEN `ci`)
   \\ simp [PULL_EXISTS]
-  \\ qexists_tac `eval_config_cfg_compile the_ev`
-  \\ qexists_tac `the_ev.encode_v c'`
+  \\ qexists_tac `adj`
+  \\ qexists_tac `the_ev with init_state :=
+        (c',THE (v_rel_conc the_ev.config_v_rel c'))`
   \\ simp [CONJ_ASSOC]
   \\ conj_asm1_tac
+
   >- (
-    simp [source_evalProofTheory.init_eval_state_def, eval_config_to_eval_state_def]
+    simp [source_evalProofTheory.precond_eval_state_def, source_evalProofTheory.mk_init_eval_state_def]
     \\ fs [prim_sem_env_eq, GSYM namespaceTheory.nsEmpty_def]
     \\ rw []
+    >- (
+
+      fs [markerTheory.Abbrev_def, opt_eval_config_wf_def]
+      fs [markerTheory.Abbrev_def, source_evalProofTheory.orac_extended_wf_def, opt_eval_config_wf_def]
+      \\ simp [FORALL_PROD]
+      \\ simp [UNCURRY, source_evalProofTheory.mk_compiler_fun_from_ci_def]
+      \\ simp [PULL_EXISTS, cake_orac_SUC, compile_inc_progs_src_env, compile_inc_progs_st_fun_def]
+      \\ rveq \\ fs []
+      \\ fs [cake_orac_def]
+      \\ rpt (gen_tac ORELSE disch_tac)
+      \\ rpt (pairarg_tac \\ fs [])
+      \\ rveq \\ fs []
+      \\ rveq \\ fs []
+    )
+
+(* saved *)
+
+    \\ fs [markerTheory.Abbrev_def,
+        source_evalProofTheory.adj_orac_respects_def]
+    \\ GEN_TAC
+    \\ disch_tac
+    \\ Induct
+    >- (
+      simp [cake_orac_0, FORALL_PROD, compile_inc_progs_src_env]
+      \\ rw [] \\ rfs []
+    )
+    \\ simp [cake_orac_SUC, FORALL_PROD, GSYM quantHeuristicsTheory.IS_SOME_EQ_NOT_NONE, IS_SOME_EXISTS, PULL_EXISTS]
+    \\ simp [source_evalProofTheory.mk_compiler_fun_from_ci_def, PULL_EXISTS, FORALL_PROD]
+    \\ rw []
+    \\ rpt (pairarg_tac \\ fs [])
+    \\ fs [compile_inc_progs_src_env]
+    \\ rveq \\ fs []
+
+cheat
+
+\\ simp [cake_orac_SUC, FORALL_PROD, GSYM quantHeuristicsTheory.IS_SOME_EQ_NOT_NONE, IS_SOME_EXISTS, PULL_EXISTS]
+\\ simp [source_evalProofTheory.mk_compiler_fun_from_ci_def, PULL_EXISTS, FORALL_PROD]
+\\ simp [UNCURRY]
+
+    \\ simp [cake_orac_def, FORALL_PROD, source_evalProofTheory.mk_compiler_fun_from_ci_def, GSYM quantHeuristicsTheory.IS_SOME_EQ_NOT_NONE, IS_SOME_EXISTS, PULL_EXISTS, EXISTS_PROD]
+    \\ rw []
+    \\ rfs []
+    \\ fs []
+
+
+
     \\ imp_res_tac eval_config_compilers_equiv
     \\ fs [match_decode_config_def, opt_eval_config_wf_def]
   )
@@ -2885,7 +2968,7 @@ Proof
     \\ rveq \\ fs []
     \\ simp [source_to_flatProofTheory.src_orac_step_invs_def]
     \\ fs [Q.ISPEC `SOME _` EQ_SYM_EQ]
-    \\ fs [eval_config_to_interp_def, K_same_type_def]
+    \\ fs [eval_config_to_interp_def]
     \\ simp [config_tuple1_def]
     \\ simp [compile_inc_progs_def, UNCURRY]
     \\ simp [source_to_flatTheory.inc_compile_def, UNCURRY]
@@ -2897,7 +2980,7 @@ Proof
     \\ simp [source_to_flatProofTheory.orac_rel_def]
     \\ qexists_tac `eval_config_compile the_ev`
     \\ simp [source_to_flatProofTheory.orac_rel_inner_def, mk_flat_install_conf_def]
-    \\ simp [eval_config_to_interp_def, K_same_type_def]
+    \\ simp [eval_config_to_interp_def]
     \\ simp [state_co_def, UNCURRY]
     \\ simp [GSYM quantHeuristicsTheory.IS_SOME_EQ_NOT_NONE, IS_SOME_EXISTS]
     \\ conj_tac
@@ -2928,7 +3011,7 @@ Proof
     \\ fs [markerTheory.Abbrev_def]
     \\ rveq \\ fs []
     \\ simp [source_to_flatProofTheory.src_orac_next_cfg_inner_def,
-        eval_config_to_interp_def, K_same_type_def]
+        eval_config_to_interp_def]
     \\ simp [config_tuple1_def]
     \\ fs [backendTheory.compile_def, compile_tap_def, source_to_flatTheory.compile_def]
     \\ rpt (pairarg_tac \\ fs [])
